Started full recursion

theories/recursion.v
@@ -102,3 +102,116 @@ Proof.
   - apply Preturn.
     reflexivity.
 Qed.
+
+(************************************************************************************)
+
+Inductive Prog (A B : Type) : Type :=
+| Ret : B -> Prog A B
+| Rec : A -> (B -> Prog A B) -> Prog A B.
+
+Inductive runProgR {A B : Type} (def : A -> Prog A B) : Prog A B -> B -> Prop :=
+| retR : forall b, runProgR def (Ret _ _ b) b
+| recR : forall a b1 b2 rest,
+    runProgR def (def a) b1
+    -> runProgR def (rest b1) b2
+    -> runProgR def (Rec _ _ a rest) b2.
+
+Theorem runProgFunction {A B : Type} {def : A -> Prog A B} {p : Prog A B} {b1 b2 : B}
+        (rp1 : runProgR def p b1) (rp2 : runProgR def p b2) : b1 = b2.
+Proof.
+  intros.
+  generalize dependent b2.
+  induction rp1.
+  - intros.
+    inversion rp2.
+    reflexivity.
+  - intros.
+    inversion rp2.
+    subst.
+    specialize (IHrp1_1 _ H1).
+    subst.
+    specialize (IHrp1_2 _ H3).
+    subst.
+    reflexivity.
+Qed.
+
+Definition runProgImpl {A B : Type} (def : A -> Prog A B) (p : Prog A B) : Classical (option B).
+  refine (choose _ (fun ob => (exists b, ob = Some b /\ runProgR def p b)
+                              \/
+                                (ob = None /\ ~ exists b, runProgR def p b)) _ _).
+  - apply (Pbind (Plem (exists b, runProgR def p b))).
+    intros H.
+    apply Preturn.
+    destruct H as [[b r] | nr].
+    + exists (Some b).
+      apply or_introl.
+      exists b.
+      auto.
+    + exists None.
+      apply or_intror.
+      auto.
+  - intros x y [H1 H2].
+    destruct H1, H2.
+    + destruct H as [b1 [p1 r1]].
+      destruct H0 as [b2 [p2 r2]].
+      subst.
+      apply f_equal.
+      apply (runProgFunction r1 r2).
+    + destruct H as [b1 [p1 r1]].
+      destruct H0 as [p2 r2].
+      destruct r2.
+      exists b1.
+      assumption.
+    + destruct H0 as [b1 [p1 r1]].
+      destruct H as [p2 r2].
+      destruct r2.
+      exists b1.
+      assumption.
+    + destruct H, H0.
+      subst.
+      reflexivity.
+Defined.
+
+Definition runProg {A B : Type} (def : A -> Prog A B) (a : A) : Classical (option B) :=
+  runProgImpl def (def a).
+
+Theorem runProgDefinitionRet {A B : Type} (def : A -> Prog A B) (b : B)
+  : PClassical (runProgImpl def (Ret _ _ b) = Creturn (Some b)).
+Proof.
+  Check choiceInd.
+  apply (choiceInd _ _ (fun x => x = Creturn (Some b))).
+  intros ob H.
+  apply Preturn.
+  destruct ob.
+  - destruct H.
+    + destruct H.
+      destruct H.
+      inversion H.
+      subst.
+      inversion H0.
+      subst.
+      reflexivity.
+    + destruct H.
+      inversion H.
+  - destruct H.
+    + destruct H.
+      destruct H.
+      inversion H.
+    + destruct H.
+      destruct H0.
+      exists b.
+      constructor.
+Qed.
+
+Definition bind {A B : Type} (a : option A) (f : A -> option B) : option B.
+Admitted.
+
+(* I probably need a monad transormer? *)
+
+Theorem runProgDefinitionRec {A B : Type} (def : A -> Prog A B) (a : A)
+        (rest : B -> Prog A B)
+  : PClassical (runProgImpl def (Rec _ _ a rest) =
+                  Cbind (runProgImpl def (def a)) (fun ob =>
+                  bind ob (fun b =>
+                  Cbind 
+               (*runProgImpl def (rest b))).*)
