theories/nodoublenegation/nodnbase.v
@@ -1,0 +1,223 @@
+(* In this file, I'm testing why I needed CProp *)
+
+Require Import Coq.Logic.ProofIrrelevance.
+(* Instead of using SProp, for now I'll just use the proof irrelevance axiom.
+   I'll see if this causes any issues; probably not. *)
+Require Import FunctionalExtensionality.
+Require Import Coq.Logic.PropExtensionality.
+
+(*
+In this versin of the monad for choice, I'm going to try making a special type of propositions that
+are all in the double negation monad.
+Following specialprop.agda
+ *)
+
+Definition PClassical (P : Prop) : Prop := not (not P).
+
+Definition Preturn {A : Prop} (x : A) : PClassical A.
+Proof.
+  intro na.
+  apply na.
+  apply x.
+Qed.
+
+Theorem Pbind {A B : Prop} (pa : PClassical A) (f : A -> PClassical B) : PClassical B.
+  Proof.
+  unfold PClassical in *.
+  intros nb.
+  apply pa.
+  intro a.
+  apply f.
+  - apply a.
+  - apply nb.
+Qed.
+
+Ltac pbind H := apply (Pbind H); clear H; intros H.
+
+Theorem sigEq :
+  forall A P S1 S2 p1 p2,
+    S1 = S2 -> @eq {a : A | P a} (exist _ S1 p1) (exist _ S2 p2).
+Proof.
+  intros.
+  subst S1.
+  assert (p1 = p2).
+  apply proof_irrelevance.
+  subst p1.
+  reflexivity.
+Qed.
+
+Theorem sigEq2:
+  forall A P (x y : {a : A | P a}), proj1_sig x = proj1_sig y -> x = y.
+Proof.
+  intros.
+  destruct x.
+  destruct y.
+  simpl in H.
+  apply sigEq.
+  assumption.
+Qed.
+
+Theorem Plem (P : Prop) : PClassical (P \/ ~P).
+Proof.
+  intros n.
+  apply n.
+  apply or_intror.
+  intros p.
+  apply n.
+  apply or_introl.
+  apply p.
+Qed.
+
+(* The "Unique" monad, that represents a unique thing that exists non-constructively *)
+Definition Classical (A : Type) : Type :=
+  {S : A -> Prop | (exists a, S a)
+                    /\ (forall x y, S x /\ S y -> x = y)}.
+
+Definition Creturn {A : Type} (x : A) : Classical A.
+  refine (exist _ (fun y => y = x) _).
+  split.
+  - exists x.
+    reflexivity.
+  - intros.
+    destruct H.
+    subst.
+    reflexivity.
+Defined.
+
+(* In this version, we really get x = y!!! *)
+Theorem CreturnInj : forall A (x y : A), Creturn x = Creturn y -> x = y.
+Proof.
+  intros.
+  pose (@f_equal _ _ (@proj1_sig _ _) _ _ H) as fact.
+  simpl in fact.
+  assert (((fun y => ((y = x))) x)). {
+    reflexivity.
+  }
+  rewrite fact in H0.
+  assumption.
+Qed.
+
+Definition Cbind {A B : Type} (pa : Classical A) (f : A -> Classical B) : Classical B.
+  refine (exist _ (fun b =>  (exists a, (proj1_sig pa a) /\ (proj1_sig (f a) b))) _).
+  destruct pa as [Sa [nonempty same]].
+  simpl.
+  split.
+  - destruct nonempty.
+    remember (f x) as fx.
+    destruct fx as [x0 [p sfsdfd]].
+    destruct p.
+    exists x1.
+    exists x.
+    split; auto.
+    rewrite <- Heqfx.
+    simpl.
+    assumption.
+  - intros x y [allx ally].
+    specialize allx as [ax [Saax fax]].
+    specialize ally as [ay [Saay fay]].
+    specialize (same _ _ (conj Saax Saay)).
+    subst.
+    apply ((proj2 (proj2_sig (f ay)) _ _ (conj fax fay))).
+Defined.
+
+(* one of the monad laws *)
+Theorem bindDef : forall A B (a : A) (f : A -> Classical B),
+    Cbind (Creturn a) f = f a.
+Proof.
+  intros.
+  apply sigEq2.
+  simpl.
+  extensionality b.
+  apply propositional_extensionality.
+  split.
+  - intros.
+    simpl in H.
+    destruct H.
+    destruct H.
+    subst.
+    assumption.
+  - intros.
+    simpl.
+    exists a.
+    split; auto.
+Qed.
+
+Theorem monadlaw2 (T : Type) (t : Classical T) : Cbind t Creturn = t.
+Proof.
+  apply sigEq2.
+  extensionality x.
+  simpl.
+  apply propositional_extensionality.
+  split.
+  - intros.
+    simpl in *.
+    destruct H as [a [ta p]].
+    subst.
+    assumption.
+  - intros.
+    simpl in *.
+    exists x.
+    split; auto.
+Qed.
+
+(* Can I get this for this version? *)
+Theorem ClassicalInd T (t : Classical T)
+  : exists x, Creturn x = t /\ (proj1_sig t x).
+Proof.
+  destruct t as [St [nonempty same]].
+  destruct nonempty as [a ta].
+  exists a.
+  split.
+  - 
+    apply sigEq2.
+    simpl.
+    extensionality t.
+    apply propositional_extensionality.
+    split.
+    + simpl.
+      intros.
+      subst.
+      assumption.
+    + intros.
+      simpl.
+      specialize (same _ _ (conj ta H)).
+      subst.
+      reflexivity.
+  - simpl.
+    assumption.
+Qed.
+
+(* unique choice *)
+Definition choose (T : Type) (P : T -> Prop)
+           (nonempty : (exists t, P t))
+           (unique : forall x y, P x /\ P y -> x = y)
+  : Classical T.
+  refine (exist _ P _).
+  split.
+  - simpl.
+    specialize nonempty as [t Pt].
+    exists t.
+    assumption.
+  - intros x y [Px Py].
+    simpl in *.
+    specialize (unique _ _ (conj Px Py)).
+    assumption.
+Defined.
+
+(* This is the exact same thing as ClassicalInd... *)
+Theorem choiceInd : forall (T : Type) (P : T -> Prop) (Q : Classical T -> Prop)
+                            nonempty unique,
+    (forall t, P t -> Q (Creturn t))
+    -> Q (@choose T P nonempty unique).
+Proof.
+  intros.
+  assert (x := (ClassicalInd _ (choose T P nonempty unique))).
+  simpl.
+  specialize x as [St [eq PSt]].
+  rewrite <- eq.
+  clear eq.
+  destruct nonempty as [t Pt].
+  specialize (H _ Pt).
+  rewrite <- (unique _ _ (conj Pt PSt)).
+  assumption.
+Qed.
